src/M/Marlowe/Semantics/Act.lean
@@ -1,7 +1,6 @@
 
 
 import M.Marlowe.Language
-import M.Marlowe.Primitives
 import Std
 
 
@@ -11,13 +10,12 @@ namespace Marlowe.Semantics
 open Marlowe.Language.Contract
 open Marlowe.Language.Input
 open Marlowe.Language.State
-open Marlowe.Primitives (Integer)
 open Std.RBMap (findD insert)
 
 
-private def deposit (s : Accounts) (a : AccountId) (t : TokenT) (n : Integer): Accounts :=
+private def deposit (s : Accounts) (a : AccountId) (t : TokenT) (n : Int): Accounts :=
   let previous := s.findD (a, t) default
-  s.insert (a, t) {toInt := previous.toInt + n.toInt}
+  s.insert (a, t) (previous + n)
 
 
 def act (s : State) : InputContent → State
