src/M/Plutus.lean
@@ -1,0 +1,9 @@
+
+
+import M.Plutus.V1.Ledger.Time
+
+
+namespace Plutus
+
+
+end Plutus
