src/M/Plutus/V1/Ledger/Time.lean
@@ -1,0 +1,38 @@
+
+
+namespace Plutus.V1.Ledger.Time
+
+
+structure POSIXTime :=
+  getPOSIXTime : Int
+deriving BEq, Inhabited, Ord, Repr
+
+
+instance : LT POSIXTime where
+  lt x y := x.getPOSIXTime < y.getPOSIXTime
+
+
+def POSIXTime.decLt (x y : POSIXTime) : Decidable (x < y) :=
+  match x, y with
+  | ⟨x⟩, ⟨y⟩ => inferInstanceAs $ Decidable (x < y)
+
+instance (x y : POSIXTime) : Decidable (x < y) :=
+  POSIXTime.decLt x y
+
+
+instance : LE POSIXTime where
+  le x y := x.getPOSIXTime <= y.getPOSIXTime
+
+
+def POSIXTime.decLe (x y : POSIXTime) : Decidable (x <= y) :=
+  match x, y with
+  | ⟨x⟩, ⟨y⟩ => inferInstanceAs $ Decidable (x <= y)
+
+instance (x y : POSIXTime) : Decidable (x <= y) :=
+  POSIXTime.decLe x y
+
+
+export POSIXTime (getPOSIXTime)
+
+
+end Plutus.V1.Ledger.Time
